theories/opsem.v
@@ -154,7 +154,7 @@ Inductive reduce : host_state -> store_record -> frame -> list administrative_in
       reduce hs s f [::AI_basic (BI_ref_func x)] hs s f [::AI_ref addr]
   | r_block :
     forall hs s f vs es n m tb t1s t2s,
-      expand f.(f_inst) tb = Some (Tf t1s t2s) ->
+      expand f.(f_inst) tb = Some (CT_func (Tf t1s t2s)) ->
       const_list vs ->
       length vs = n ->
       length t1s = n ->
@@ -162,7 +162,7 @@ Inductive reduce : host_state -> store_record -> frame -> list administrative_in
       reduce hs s f (vs ++ [::AI_basic (BI_block tb es)]) hs s f [::AI_label m [::] (vs ++ to_e_list es)]
   | r_loop :
       forall hs s f vs es n m tb t1s t2s,
-      expand f.(f_inst) tb = Some (Tf t1s t2s) ->
+      expand f.(f_inst) tb = Some (CT_func (Tf t1s t2s)) ->
       const_list vs ->
       length vs = n ->
       length t1s = n ->
@@ -177,13 +177,13 @@ Inductive reduce : host_state -> store_record -> frame -> list administrative_in
       forall s f x (y: typeidx) a cl i hs,
         stab_elem s f.(f_inst) x (Wasm_int.N_of_uint i32m i) = Some (VAL_ref_func a) ->
         lookup_N s.(s_funcs) a = Some cl ->
-        lookup_N f.(f_inst).(inst_types) y = Some (cl_type cl) ->
+        lookup_N f.(f_inst).(inst_types) y = Some (CT_func (cl_type cl)) ->
         reduce hs s f [::$VN (VAL_int32 i); AI_basic (BI_call_indirect x y)] hs s f [::AI_invoke a]
   | r_call_indirect_failure_mismatch :
       forall s f x (y: typeidx) a cl i hs,
         stab_elem s f.(f_inst) x (Wasm_int.N_of_uint i32m i) = Some (VAL_ref_func a) ->
         lookup_N s.(s_funcs) a = Some cl ->
-        lookup_N f.(f_inst).(inst_types) y <> Some (cl_type cl) ->
+        lookup_N f.(f_inst).(inst_types) y <> Some (CT_func (cl_type cl)) ->
         reduce hs s f [::$VN (VAL_int32 i); AI_basic (BI_call_indirect x y)] hs s f [::AI_trap]
   | r_call_indirect_failure_bound :
       forall s f x (y: typeidx) i hs,
